inst progress and reorg

theories/iris/logrel/env_props.v
@@ -4,6 +4,7 @@ Require Import RichWasm.iris.logrel.
 Require Import RichWasm.layout.
 Require Import RichWasm.syntax.
 Require Import RichWasm.typing.
+Require Import RichWasm.util.
 Set Bullet Behavior "Strict Subproofs".
 Set Default Goal Selector "!".
 
@@ -13,6 +14,8 @@ Section env_props.
   Context `{!wasmG Σ}.
   Context `{!richwasmG Σ}.
 
+  (* note: first half of file is 10 billion eval insertion/substitution
+     for lemmas related to actually inserting into, search INSERTION LEMMAS *)
 
   Lemma eval_rep_mem_irrel_eq se ρ μ :
     eval_rep se ρ =
@@ -186,6 +189,390 @@ Section env_props.
   Proof.
     intros; rewrite <- type_skind_mem_irrel_eq; done.
   Qed.
+
+
+  Definition mem_ok_se (se : semantic_env) (μ : Core.memory) : Prop :=
+    match μ with
+    | VarM i => i < length (senv_mems (Σ:=Σ) se)
+    | BaseM _ => True
+    end.
+
+  Lemma mem_ok_se_up_mem μ se sub_m i :
+    mem_ok_se se (sub_m i) <->
+      mem_ok_se (senv_insert_mem μ se) (up_memory_memory sub_m (S i)).
+  Proof.
+    unfold mem_ok_se.
+    assert (Hope: ren_memory unscoped.shift (sub_m i) = up_memory_memory sub_m (S i)) by by substify.
+    split.
+    {
+      intros H.
+      rewrite <- Hope.
+      cbn.
+      destruct (sub_m i) eqn:Hsubi.
+      - cbn. unfold unscoped.shift. cbn in H. lia.
+      - cbn. auto.
+    }
+    {
+      intros H.
+      rewrite <- Hope in H.
+      cbn in *.
+      destruct (sub_m i) eqn:Hsubi.
+      - cbn in H. unfold unscoped.shift in H. lia.
+      - auto.
+    }
+  Qed.
+
+  Lemma mem_ok_se_up_rep ρ se sub_m i :
+    mem_ok_se se (sub_m i) <->
+      mem_ok_se (senv_insert_rep ρ se) (up_representation_memory sub_m i).
+  Proof.
+    unfold mem_ok_se.
+    split.
+    {
+      intros H.
+      unfold up_representation_memory, core.funcomp.
+      by rewrite rinstId'_memory.
+    }
+    {
+      intros H.
+      unfold up_representation_memory, core.funcomp in H.
+      by rewrite rinstId'_memory in H.
+    }
+  Qed.
+
+  Lemma mem_ok_se_up_size ρ se sub_m i :
+    mem_ok_se se (sub_m i) <->
+      mem_ok_se (senv_insert_size ρ se) (up_size_memory sub_m i).
+  Proof.
+    unfold mem_ok_se.
+    split.
+    {
+      intros H.
+      unfold up_size_memory, core.funcomp.
+      by rewrite rinstId'_memory.
+    }
+    {
+      intros H.
+      unfold up_size_memory, core.funcomp in H.
+      by rewrite rinstId'_memory in H.
+    }
+  Qed.
+
+  Lemma mem_ok_se_up_type sκ sκ_T T se sub_m i :
+    mem_ok_se se (sub_m i) <->
+      mem_ok_se (senv_insert_type sκ sκ_T T se) (up_type_memory sub_m i).
+  Proof.
+    unfold mem_ok_se.
+    split.
+    {
+      intros H.
+      unfold up_type_memory, core.funcomp.
+      by rewrite rinstId'_memory.
+    }
+    {
+      intros H.
+      unfold up_type_memory, core.funcomp in H.
+      by rewrite rinstId'_memory in H.
+    }
+  Qed.
+
+  (* moved type_skind_has_kind_Some to kinding.v *)
+
+  Ltac shred_for_up_mini n2 Hn2 :=
+      apply fmap_Some;
+      exists n2; split; last done;
+      apply mapM_Some in Hn2;
+      apply mapM_Some;
+      eapply Forall2_mini_impl_Forall; first done;
+      done.
+  Ltac shred_for_up n2 Hn2 :=
+      apply fmap_Some;
+      exists n2; split; last done;
+      apply mapM_Some in Hn2;
+      apply mapM_Some;
+      rewrite <- (list_fmap_id n2);
+      rewrite map_fmap;
+      apply Forall2_fmap;
+      eapply Forall2_mini_impl_Forall; first done;
+      done.
+
+  Lemma eval_rep_up_rep_eq se sub_r ιs0 i :
+    eval_rep se (sub_r i) =
+    eval_rep (senv_insert_rep (Σ:=Σ) ιs0 se) (up_representation_representation sub_r (S i)).
+  Proof.
+    asimpl'.
+    unfold core.funcomp.
+    induction (sub_r i) using rep_ind; try (by cbn).
+    - Opaque senv_insert_rep.
+      cbn.
+      assert (H': mapM (eval_rep se) ρs = mapM (eval_rep (senv_insert_rep ιs0 se))
+             (map (ren_representation unscoped.shift) ρs)) by (by apply Forall_mapM_map_ext).
+      by rewrite H'.
+    - cbn.
+      assert (H': mapM (eval_rep se) ρs = mapM (eval_rep (senv_insert_rep ιs0 se))
+             (map (ren_representation unscoped.shift) ρs)) by (by apply Forall_mapM_map_ext).
+      by rewrite H'.
+  Qed.
+
+  Lemma eval_rep_up_rep se sub_r ιs0 i ιs :
+    eval_rep se (sub_r i) = Some ιs ->
+    eval_rep (senv_insert_rep (Σ:=Σ) ιs0 se) (up_representation_representation sub_r (S i)) = Some ιs.
+  Proof.
+    intros; rewrite <- eval_rep_up_rep_eq; done.
+  Qed.
+
+  Lemma eval_rep_up_size_eq se sub_r i n :
+    eval_rep se (sub_r i) =
+    eval_rep (senv_insert_size (Σ:=Σ) n se) (up_size_representation sub_r i).
+  Proof.
+    asimpl'.
+    unfold core.funcomp.
+    by rewrite <- eval_rep_size_irrel_eq.
+  Qed.
+
+  Lemma eval_rep_up_size se sub_r ιs i n :
+    eval_rep se (sub_r i) = Some ιs ->
+    eval_rep (senv_insert_size (Σ:=Σ) n se) (up_size_representation sub_r i) = Some ιs.
+  Proof.
+    asimpl'.
+    by apply eval_rep_size_irrel.
+  Qed.
+
+  Lemma eval_rep_up_memory_eq se sub_r i μ :
+    eval_rep se (sub_r i) =
+    eval_rep (senv_insert_mem (Σ:=Σ) μ se) (up_memory_representation sub_r i).
+  Proof.
+    asimpl'.
+    unfold core.funcomp.
+    by rewrite <- eval_rep_mem_irrel_eq.
+  Qed.
+
+  Lemma eval_rep_up_type_eq se sub_r i sκ sκ_T T :
+    eval_rep se (sub_r i) =
+    eval_rep (senv_insert_type (Σ:=Σ) sκ sκ_T T se) (up_type_representation sub_r i).
+  Proof.
+    asimpl'.
+    unfold core.funcomp.
+    by rewrite <- eval_rep_type_irrel_eq.
+  Qed.
+
+  Lemma eval_rep_up_memory se sub_r ιs i μ :
+    eval_rep se (sub_r i) = Some ιs ->
+    eval_rep (senv_insert_mem (Σ:=Σ) μ se) (up_memory_representation sub_r i) = Some ιs.
+  Proof.
+    asimpl'.
+    by apply eval_rep_mem_irrel.
+  Qed.
+
+  Lemma eval_size_up_memory_eq se sub_s i μ :
+    eval_size se (sub_s i) =
+    eval_size (senv_insert_mem (Σ:=Σ) μ se) (up_memory_size sub_s i).
+  Proof.
+    asimpl'.
+    unfold core.funcomp.
+    by rewrite <- eval_size_mem_irrel_eq.
+  Qed.
+
+  Lemma eval_size_up_memory se sub_s n i μ :
+    eval_size se (sub_s i) = Some n ->
+    eval_size (senv_insert_mem (Σ:=Σ) μ se) (up_memory_size sub_s i) = Some n.
+  Proof.
+    asimpl'.
+    by apply eval_size_mem_irrel.
+  Qed.
+
+  Lemma eval_size_up_type_eq se sub_s i sκ sκ_T T :
+    eval_size se (sub_s i) =
+    eval_size (senv_insert_type (Σ:=Σ) sκ sκ_T T se) (up_type_size sub_s i).
+  Proof.
+    asimpl'.
+    unfold core.funcomp.
+    by rewrite <- eval_size_type_irrel_eq.
+  Qed.
+
+  Lemma eval_mem_up_type_eq se sub_m i sκ sκ_T T :
+    eval_mem se (sub_m i) =
+    eval_mem (senv_insert_type (Σ:=Σ) sκ sκ_T T se) (up_type_memory sub_m i).
+  Proof.
+    asimpl'.
+    unfold core.funcomp.
+    by rewrite <- eval_mem_type_irrel_eq.
+  Qed.
+
+  Lemma eval_mem_up_shift_mem_eq se μ mm :
+    eval_mem se mm =
+    eval_mem (senv_insert_mem (Σ:=Σ) μ se) (ren_memory unscoped.shift mm).
+  Proof.
+    destruct mm; by cbn.
+  Qed.
+
+  Lemma eval_rep_up_shift_rep_eq se ρ ιs :
+    eval_rep se ρ =
+    eval_rep (senv_insert_rep (Σ:=Σ) ιs se) (ren_representation unscoped.shift ρ) .
+  Proof.
+    induction ρ using rep_ind; try (by cbn).
+    - cbn.
+      assert (H': mapM (eval_rep se) ρs = mapM (eval_rep (senv_insert_rep ιs se))
+             (map (ren_representation unscoped.shift) ρs)) by (by apply Forall_mapM_map_ext).
+      by rewrite H'.
+    - cbn.
+      assert (H': mapM (eval_rep se) ρs = mapM (eval_rep (senv_insert_rep ιs se))
+             (map (ren_representation unscoped.shift) ρs)) by (by apply Forall_mapM_map_ext).
+      by rewrite H'.
+  Qed.
+
+  Lemma eval_rep_up_shift_rep se ρ n ιs :
+    eval_rep se ρ = Some n ->
+    eval_rep (senv_insert_rep (Σ:=Σ) ιs se) (ren_representation unscoped.shift ρ) = Some n.
+  Proof.
+    rewrite <- eval_rep_up_shift_rep_eq. done.
+  Qed.
+
+  Lemma eval_size_up_shift_rep_eq se σ ιs :
+    eval_size se σ =
+    eval_size (senv_insert_rep (Σ:=Σ) ιs se) (ren_size unscoped.shift unscoped.id σ) .
+  Proof.
+    induction σ using size_ind; try (by cbn).
+    - cbn.
+      assert (H': mapM (eval_size se) σs = mapM (eval_size (senv_insert_rep ιs se))
+             (map (ren_size unscoped.shift unscoped.id) σs)) by (by apply Forall_mapM_map_ext).
+      by rewrite H'.
+    - cbn.
+      assert (H': mapM (eval_size se) σs = mapM (eval_size (senv_insert_rep ιs se))
+             (map (ren_size unscoped.shift unscoped.id) σs)) by (by apply Forall_mapM_map_ext).
+      by rewrite H'.
+    - cbn. by rewrite <- eval_rep_up_shift_rep_eq.
+  Qed.
+
+  Lemma eval_size_up_shift_size_eq se n σ :
+    eval_size se σ =
+      eval_size (senv_insert_size (Σ:=Σ) n se) (ren_size unscoped.id unscoped.shift σ).
+  Proof.
+    induction σ using size_ind; try by cbn.
+    - cbn.
+      assert (H': mapM (eval_size se) σs = mapM (eval_size (senv_insert_size n se))
+             (map (ren_size unscoped.id unscoped.shift) σs)) by (by apply Forall_mapM_map_ext).
+      by rewrite H'.
+    - cbn.
+      assert (H': mapM (eval_size se) σs = mapM (eval_size (senv_insert_size n se))
+             (map (ren_size unscoped.id unscoped.shift) σs)) by (by apply Forall_mapM_map_ext).
+      by rewrite H'.
+    - cbn -[senv_insert_size].
+      rewrite rinstId'_representation.
+      by rewrite <- eval_rep_size_irrel_eq.
+  Qed.
+
+  Lemma eval_size_up_shift_rep se ρ n ιs :
+    eval_rep se ρ = Some n ->
+    eval_rep (senv_insert_rep (Σ:=Σ) ιs se) (ren_representation unscoped.shift ρ) = Some n.
+  Proof.
+    rewrite <- eval_rep_up_shift_rep_eq. done.
+  Qed.
+
+  Lemma eval_size_up_rep_eq se sub_s ιs i :
+    eval_size se (sub_s i) =
+    eval_size (senv_insert_rep (Σ:=Σ) ιs se) (up_representation_size sub_s i).
+  Proof.
+    asimpl'; unfold core.funcomp.
+    induction (sub_s i) using size_ind; try (by cbn).
+    - cbn.
+      assert (H': mapM (eval_size se) σs = mapM (eval_size (senv_insert_rep ιs se))
+             (map (ren_size unscoped.shift unscoped.id) σs)) by (by apply Forall_mapM_map_ext).
+      by rewrite H'.
+    - cbn.
+      assert (H': mapM (eval_size se) σs = mapM (eval_size (senv_insert_rep ιs se))
+             (map (ren_size unscoped.shift unscoped.id) σs)) by (by apply Forall_mapM_map_ext).
+      by rewrite H'.
+    - cbn.
+      by rewrite <- eval_rep_up_shift_rep_eq.
+  Qed.
+
+  Lemma eval_size_up_rep se sub_s ιs i n :
+    eval_size se (sub_s i) = Some n ->
+    eval_size (senv_insert_rep (Σ:=Σ) ιs se) (up_representation_size sub_s i) = Some n.
+  Proof.
+    intros H.
+    rewrite <- eval_size_up_rep_eq; done.
+  Qed.
+
+  Lemma eval_kind_up_shift_rep_eq se κ ιs :
+    eval_kind se κ =
+    eval_kind (senv_insert_rep (Σ:=Σ) ιs se) (ren_kind unscoped.shift unscoped.id κ) .
+  Proof.
+    induction κ as [ρ ξ | σ ξ].
+    - cbn. by rewrite <- eval_rep_up_shift_rep_eq.
+    - cbn. by rewrite <- eval_size_up_shift_rep_eq.
+  Qed.
+
+  Lemma eval_kind_up_shift_size_eq se κ n:
+    eval_kind se κ =
+    eval_kind (senv_insert_size (Σ:=Σ) n se) (ren_kind unscoped.id unscoped.shift κ) .
+  Proof.
+    induction κ as [ρ ξ | σ ξ].
+    - cbn -[senv_insert_size].
+      rewrite rinstId'_representation.
+      by rewrite <- eval_rep_size_irrel_eq.
+    - cbn -[senv_insert_size].
+      by rewrite <- eval_size_up_shift_size_eq.
+  Qed.
+
+  Lemma eval_kind_up_shift_rep se κ sκ ιs :
+    eval_kind se κ = Some sκ ->
+    eval_kind (senv_insert_rep (Σ:=Σ) ιs se) (ren_kind unscoped.shift unscoped.id κ) = Some sκ.
+  Proof.
+    by rewrite <- eval_kind_up_shift_rep_eq.
+  Qed.
+
+  Lemma type_skind_up_rep_eq se sub_t ιs i :
+    type_skind se (sub_t i) =
+    type_skind (Σ:=Σ) (senv_insert_rep ιs se) (up_representation_type sub_t i) .
+  Proof.
+    asimpl'; unfold core.funcomp.
+    induction (sub_t i) using type_ind with (P0 := λ ft, True) (Pi := λ ft, True);
+      cbn in *; auto; by apply eval_kind_up_shift_rep_eq.
+  Qed.
+
+  Lemma type_skind_up_rep se sub_t ιs sκ i :
+    type_skind se (sub_t i) = Some sκ ->
+    type_skind (Σ:=Σ) (senv_insert_rep ιs se) (up_representation_type sub_t i) = Some sκ.
+  Proof.
+    by rewrite <- type_skind_up_rep_eq.
+  Qed.
+
+  Lemma type_skind_up_memory_eq se sub_t μ i :
+    type_skind se (sub_t i) =
+    type_skind (Σ:=Σ) (senv_insert_mem μ se) (up_memory_type sub_t i) .
+  Proof.
+    asimpl'; unfold core.funcomp.
+    induction (sub_t i) using type_ind with (P0 := λ ft, True) (Pi := λ ft, True);
+      cbn in *; auto; rewrite rinstId'_kind; by apply eval_kind_mem_irrel_eq.
+  Qed.
+
+  Lemma type_skind_up_memory se sub_t μ sκ i :
+    type_skind se (sub_t i) = Some sκ ->
+    type_skind (Σ:=Σ) (senv_insert_mem μ se) (up_memory_type sub_t i) = Some sκ.
+  Proof.
+    by rewrite <- type_skind_up_memory_eq.
+  Qed.
+
+  Lemma type_skind_up_type_eq se sub_t sκ' sκ_T T i :
+    type_skind se (sub_t i) =
+    type_skind (Σ:=Σ) (senv_insert_type sκ' sκ_T T se) (up_type_type sub_t (S i)) .
+  Proof.
+    asimpl'; unfold core.funcomp.
+    induction (sub_t i) using type_ind with (P0 := λ ft, True) (Pi := λ ft, True);
+      cbn in *; auto; rewrite rinstId'_kind; by apply eval_kind_type_irrel_eq.
+  Qed.
+
+  Lemma type_skind_up_type se sub_t sκ' sκ_T T sκ i :
+    type_skind se (sub_t i) = Some sκ ->
+    type_skind (Σ:=Σ) (senv_insert_type sκ' sκ_T T se) (up_type_type sub_t (S i)) = Some sκ.
+  Proof.
+    by rewrite <- type_skind_up_type_eq.
+  Qed.
+
+
+  (* INSERTION LEMMAS *)
 
   Lemma sem_env_interp_insert_type F (se : semantic_env (Σ:=Σ)) κ sκ sκ_T T :
     sem_env_interp F se →
