theories/util.v
@@ -689,3 +689,17 @@ Qed.
       cbn.
       lia.
   Qed.
+
+  Lemma Forall_mapM_map_ext {A B:Type} (f g:A → option B) h (l: list A) :
+    Forall (λ x, f x = g (h x)) l -> mapM f l = mapM g (map h l).
+  Proof.
+    revert l.
+    induction l.
+    - by cbn.
+    - intros.
+      apply Forall_cons_1 in H as [ha Hl].
+      apply IHl in Hl.
+      cbn.
+      rewrite ha.
+      rewrite Hl. done.
+  Qed.
